src/program_proof/tulip/tulip_proof.v
@@ -1,0 +1,2 @@
+(* paxos *)
+From Perennial.program_proof.tulip.paxos.program Require Export paxos.
