src/program_proof/tulip/util/next_aligned.v
@@ -1,0 +1,72 @@
+From Perennial.program_proof.tulip Require Import prelude.
+From Perennial.program_proof Require Import std_proof.
+From Goose.github_com.mit_pdos.tulip Require Import util.
+
+Local Ltac Zify.zify_post_hook ::= Z.div_mod_to_equations.
+
+Section next_aligned.
+  Context `{!heapGS Σ, !paxos_ghostG Σ}.
+
+  Lemma Z_next_aligned (c i l : Z) :
+    0 ≤ l < i ->
+    (c + (l - (c `mod` i))) `mod` i = l.
+  Proof.
+    intros Horder.
+    rewrite Zplus_mod Zminus_mod Zmod_mod -Zminus_mod -Zplus_mod.
+    replace (c + _) with l by lia.
+    apply Zmod_small. lia.
+  Qed.
+
+  Theorem wp_NextAligned (current : u64) (interval : u64) (low : u64) :
+    uint.Z interval < 2 ^ 63 ->
+    0 ≤ uint.Z low < uint.Z interval ->
+    {{{ True }}}
+      NextAligned #current #interval #low
+    {{{ (n : u64), RET #n;
+        ⌜uint.Z current < uint.Z n ∧ uint.Z n `mod` uint.Z interval = uint.Z low⌝
+    }}}.
+  Proof.
+    iIntros (Hitv Horder Φ) "_ HΦ".
+    wp_rec. wp_pures.
+
+    (*@ func NextAligned(current, interval, low uint64) uint64 {                @*)
+    (*@     var delta uint64                                                    @*)
+    (*@                                                                         @*)
+    wp_apply (wp_ref_of_zero); first done.
+    iIntros (deltaRef) "HdeltaRef".
+    wp_pures.
+
+    (*@     rem := current % interval                                           @*)
+    (*@     if rem < low {                                                      @*)
+    (*@         delta = low - rem                                               @*)
+    (*@     } else {                                                            @*)
+    (*@         delta = interval + low - rem                                    @*)
+    (*@     }                                                                   @*)
+    (*@     return std.SumAssumeNoOverflow(current, delta)                      @*)
+    (*@ }                                                                       @*)
+    set rem := (word.modu _ _).
+    wp_if_destruct; wp_store; wp_load; wp_apply wp_SumAssumeNoOverflow.
+    - iIntros (Hoverflow). iApply "HΦ". iPureIntro.
+      rewrite Hoverflow.
+      split; first word.
+      rewrite word.unsigned_sub_nowrap; last lia.
+      rewrite word.unsigned_modu_nowrap; last lia.
+      apply Z_next_aligned.
+      lia.
+    - iIntros (Hoverflow). iApply "HΦ". iPureIntro.
+      rewrite Hoverflow.
+      rewrite word.unsigned_sub_nowrap; last first.
+      { rewrite word.unsigned_add_nowrap; last lia.
+        rewrite word.unsigned_modu_nowrap; lia.
+      }
+      rewrite word.unsigned_add_nowrap; last lia.
+      rewrite word.unsigned_modu_nowrap; last lia.
+      rewrite word.unsigned_modu_nowrap in Heqb; last lia.
+      split; first lia.
+      rewrite -Z.add_sub_assoc Z.add_assoc (Z.add_comm (uint.Z current)) -Z.add_assoc.
+      rewrite Zplus_mod Z_mod_same_full Z.add_0_l Zmod_mod.
+      apply Z_next_aligned.
+      lia.
+  Qed.
+
+End next_aligned.
